theories/VLSM/Core/ByzantineTraces/FixedSetByzantineTraces.v
@@ -181,13 +181,9 @@ Lemma fixed_non_byzantine_projection_incl_preloaded
 Proof.
   apply basic_VLSM_strong_incl.
   - by intros s H1; apply fixed_non_byzantine_projection_initial_state_preservation.
-  - by intros m H1; cbv.
-  - by split; [eapply induced_sub_projection_valid_preservation|].
-  - intros l s om s' om'.
-    unfold vtransition, transition, machine.
-    cbn [vtransition transition machine vmachine].
-    unfold projection_induced_vlsm_machine.
-    unfold pre_loaded_with_all_messages_vlsm_machine.
+  - by intros.
+  - by split; [eapply induced_sub_projection_valid_preservation |].
+  - intros l s om s' om'; cbn.
     (* an ugly trick to get the forward direction from an iff (<->) lemma *)
     by eapply proj1; rapply @induced_sub_projection_transition_preservation.
 Qed.
@@ -444,7 +440,7 @@ Proof.
     inversion 1; itauto.
 Qed.
 
-(** Since the [fixed_non_byzantine_projection] is an [induced_projection] of
+(** Since the [fixed_non_byzantine_projection] is an [induced_validator] of
 the composition of [fixed_byzantine_IM] with a
 [non_byzantine_not_equivocating_constraint], its initial_messages and validity
 are derived from valid messages and protocol validity of the larger
@@ -471,9 +467,10 @@ Proof.
   - intros l s om Hv.
     exists (lift_sub_label fixed_byzantine_IM non_byzantine l).
     exists (lift_sub_state fixed_byzantine_IM non_byzantine s).
-    split; [apply composite_label_sub_projection_option_lift |].
-    split; [apply composite_state_sub_projection_lift |].
-    by apply (VLSM_full_projection_input_valid pre_loaded_fixed_non_byzantine_vlsm_lift).
+    split.
+    + apply composite_label_sub_projection_option_lift.
+    + apply composite_state_sub_projection_lift.
+    + by apply (VLSM_full_projection_input_valid pre_loaded_fixed_non_byzantine_vlsm_lift).
   - intros l s om s' om' [_ Ht].
     by apply induced_sub_projection_transition_preservation.
 Qed.
@@ -696,7 +693,7 @@ Context
     : weak_full_projection_initial_message_preservation PreNonByzantine Fixed
     (lift_sub_state IM (set_diff (enum index) selection))).
 
-(** Since <<FixedNonEquivocating>> is an [induced_projection] of <<Fixed>>,
+(** Since <<FixedNonEquivocating>> is an [induced_validator] of <<Fixed>>,
 its initial_messages and validity are derived from valid messages and
 protocol validity of the larger composition; therefore, the following
 result becomes very important.
@@ -726,10 +723,11 @@ Proof.
   - intros l s om Hv HsY HomY.
     exists (lift_sub_label IM (set_diff (enum index) selection) l).
     exists (lift_sub_state IM (set_diff (enum index) selection) s).
-    split; [apply composite_label_sub_projection_option_lift |].
-    split; [apply composite_state_sub_projection_lift |].
-    apply @VLSM_full_projection_input_valid; [| done].
-    apply fixed_non_byzantine_vlsm_lift_from_initial.
+    split.
+    + apply composite_label_sub_projection_option_lift.
+    + apply composite_state_sub_projection_lift.
+    + apply @VLSM_full_projection_input_valid; [| done].
+      apply fixed_non_byzantine_vlsm_lift_from_initial.
   - intros l s om s' om' [_ Ht].
     by apply induced_sub_projection_transition_preservation.
 Qed.
